proof/correctproof/correct_get_block_perm.v
@@ -1,0 +1,91 @@
+From bpf.comm Require Import MemRegion State Monad.
+From bpf.src Require Import DxValues DxInstructions.
+From dx.Type Require Import Bool.
+From dx Require Import IR.
+From Coq Require Import List ZArith.
+From compcert Require Import Integers Values Clight Memory AST.
+From compcert Require Import Coqlib.
+Import ListNotations.
+
+From bpf.proof Require Import clight_exec Clightlogic CorrectRel MatchState CommonLemma.
+
+From bpf.clight Require Import interpreter.
+
+
+(**
+Check get_block_perm.
+
+get_block_perm
+     : memory_region -> DxMonad.M permission
+*)
+
+Section Get_block_perm.
+
+  (** The program contains our function of interest [fn] *)
+  Definition p : Clight.program := prog.
+
+  (* [Args,Res] provides the mapping between the Coq and the C types *)
+  (* Definition Args : list CompilableType := [stateCompilableType].*)
+  Definition args : list Type := [(memory_region:Type)].
+  Definition res : Type := (permission:Type).
+
+  (* [f] is a Coq Monadic function with the right type *)
+  Definition f : arrow_type args (M res) := get_block_perm.
+
+  Variable state_block: block. (**r a block storing all rbpf state information? *)
+  Variable mrs_block: block.
+  Variable ins_block: block.
+
+  (* [fn] is the Cligth function which has the same behaviour as [f] *)
+  Definition fn: Clight.function := f_get_block_perm.
+
+  (* [match_arg] relates the Coq arguments and the C arguments *)
+  Definition match_arg_list : DList.t (fun x => x -> val -> State.state -> Memory.Mem.mem -> Prop) args :=
+    (DList.DCons (my_match_region mrs_block)
+       (DList.DNil _)).
+
+  (* [match_res] relates the Coq result and the C result *)
+  Definition match_res : res -> val -> State.state -> Memory.Mem.mem -> Prop := fun x v st m => perm_correct x v.
+
+  Instance correct_function3_get_block_perm : forall a, correct_function3 p args res f fn (nil) true match_arg_list match_res a.
+  Proof.
+    correct_function_from_body args.
+    correct_body.
+    (** how to use correct_* *)
+    unfold INV.
+    unfold f.
+    repeat intro.
+    get_invariant_more _mr.
+
+    unfold my_match_region in H0.
+    destruct H0 as (o & Hptr & Hmatch).
+    unfold match_region_at_ofs in Hmatch.
+    destruct Hmatch as (_ & _ & (vperm & Hperm_load & Hinj) & _).
+    subst.
+
+    (**according to the type:
+         static unsigned long long getMemRegion_start_addr(struct memory_region *mr1)
+       1. return value should be  `Vlong vaddr`
+       2. the memory is same
+      *)
+    exists (Vint vperm), m, Events.E0.
+
+    repeat split; unfold step2.
+    -
+      repeat forward_star.
+      unfold align, Ctypes.alignof; simpl.
+      unfold Mem.loadv in Hperm_load.
+      rewrite Hperm_load; reflexivity.
+
+      Transparent Archi.ptr64.
+      reflexivity.
+    - unfold match_res. unfold correct_perm in Hinj. unfold perm_correct. 
+      destruct (block_perm c); rewrite Hinj; reflexivity.
+    - simpl.
+      constructor.
+      reflexivity.
+  Qed.
+
+End Get_block_perm.
+
+Existing Instance correct_function3_get_block_perm.
