proof/correctproof/correct_get_opcode_branch.v
@@ -1,0 +1,109 @@
+From bpf.comm Require Import Regs State Monad.
+From bpf.src Require Import DxNat DxOpcode DxIntegers DxInstructions.
+From Coq Require Import List Lia ZArith.
+From compcert Require Import Integers Values Clight Memory.
+Import ListNotations.
+
+From bpf.proof Require Import Clightlogic MatchState CorrectRel CommonLemma CommonLemmaNat.
+
+From bpf.clight Require Import interpreter.
+
+
+(**
+Check get_opcode_branch.
+get_opcode_branch
+     : nat8 -> DxMonad.M opcode_branch
+
+*)
+
+Section Get_opcode_branch.
+
+  (** The program contains our function of interest [fn] *)
+  Definition p : Clight.program := prog.
+
+  (* [Args,Res] provides the mapping between the Coq and the C types *)
+  (* Definition Args : list CompilableType := [stateCompilableType].*)
+  Definition args : list Type := [(nat8:Type)].
+  Definition res : Type := (opcode_branch:Type).
+
+  (* [f] is a Coq Monadic function with the right type *)
+  Definition f : arrow_type args (M res) := get_opcode_branch.
+
+  Variable state_block: block. (**r a block storing all rbpf state information? *)
+  Variable mrs_block: block.
+  Variable ins_block: block.
+
+  (* [fn] is the Cligth function which has the same behaviour as [f] *)
+  Definition fn: Clight.function := f_get_opcode_branch.
+
+  (* [match_arg] relates the Coq arguments and the C arguments *)
+  Definition match_arg_list : DList.t (fun x => x -> val -> State.state -> Memory.Mem.mem -> Prop) args :=
+    (DList.DCons (stateless opcode_alu64_nat8_correct)
+                (DList.DNil _)).
+
+  (* [match_res] relates the Coq result and the C result *)
+  Definition match_res : res -> val -> State.state -> Memory.Mem.mem -> Prop := fun x v st m => opcode_branch_correct x v.
+
+  Instance correct_function3_get_opcode_branch : forall a, correct_function3 p args res f fn nil true match_arg_list match_res a.
+  Proof.
+    correct_function_from_body args.
+    correct_body.
+    (** how to use correct_* *)
+    unfold INV.
+    unfold f.
+    repeat intro.
+    get_invariant_more _op.
+
+    unfold stateless, opcode_alu64_nat8_correct in H0.
+    destruct H0 as (H0 & Hland & Hge).
+    subst.
+
+    eexists. exists m, Events.E0.
+
+    repeat split; unfold step2.
+    -
+      repeat forward_star.
+    - simpl.
+      (**r Search (Int.zero_ext).*)
+      rewrite Int.zero_ext_idem;[idtac | lia].
+      unfold match_res, opcode_branch_correct.
+      rewrite byte_to_opcode_branch_if_same.
+      unfold byte_to_opcode_branch_if.
+      rewrite Int.zero_ext_and; [simpl | lia].
+      rewrite nat8_land_240_255_eq; [| apply Hge].
+
+Ltac simpl_if Ht :=
+  match goal with
+  | |- context [if ?X then _ else _] =>
+    destruct X eqn: Ht; [rewrite Nat.eqb_eq in Ht | rewrite Nat.eqb_neq in Ht]
+  end.
+
+Ltac simpl_alu_opcode Hop := simpl_if Hop; [rewrite Hop; reflexivity | ].
+
+      simpl_if Hja.
+      destruct (c =? 5)%nat eqn: Hc_eq; [rewrite Nat.eqb_eq in Hc_eq; rewrite Hc_eq; reflexivity | eexists; reflexivity].
+      simpl_alu_opcode Hjeq.
+      simpl_alu_opcode Hjgt.
+      simpl_alu_opcode Hjge.
+      simpl_alu_opcode Hjlt.
+      simpl_alu_opcode Hjle.
+      simpl_alu_opcode Hjset.
+      simpl_alu_opcode Hjne.
+      simpl_alu_opcode Hjsgt.
+      simpl_alu_opcode Hjsge.
+      simpl_alu_opcode Hjsjt.
+      simpl_alu_opcode Hjsle.
+      simpl_if Hret.
+      destruct (c =? 149)%nat eqn: Hc_eq; [rewrite Nat.eqb_eq in Hc_eq; rewrite Hc_eq; reflexivity | eexists; reflexivity].
+      eexists; reflexivity.
+    - simpl.
+      constructor.
+      rewrite Int.zero_ext_idem;[idtac | lia].
+      simpl.
+      rewrite Int.zero_ext_idem;[idtac | lia].
+      reflexivity.
+Qed.
+
+End Get_opcode_branch.
+
+Existing Instance correct_function3_get_opcode_branch.
