proof/correctproof/correct_step_opcode_alu64.v
@@ -624,7 +624,7 @@ Ltac correct_forward L :=
         reflexivity.
         reflexivity.
         reflexivity.
-        admit.
+        reflexivity.
         reflexivity.
 
         unfold INV; intro H.
@@ -857,196 +857,6 @@ Ltac correct_forward L :=
       + compute. intuition congruence.
     - (**r op_BPF_LSH64 *)
       admit.
-      (*
-      eapply correct_statement_switch with (n:= 96).
-      + simpl.
-        (**r s1 -> (Ssequence s1 s2) *)
-        eapply correct_statement_seq_body_drop.
-        intros.
-        (**r correct_body p unit (bindM (reg64_to_reg32 c0) ... *)
-        eapply correct_statement_seq_body_pure.
-        change_app_for_statement.
-
-
-        eapply correct_statement_if_body_expr.
-        destruct (rBPFValues.compl_ne c0 val64_zero) eqn: Hdiv_zero.
-
-
-        eapply correct_statement_seq_body_unit.
-        change_app_for_statement.
-        (**r goal: correct_statement p unit (app f a) fn (Scall None (Evar ... *)
-        eapply correct_statement_call_none.
-        my_reflex.
-        my_reflex.
-        reflexivity.
-        typeclasses eauto.
-        unfold correct_upd_reg.match_res. intuition.
-        { unfold modifies.
-          instantiate (1:= ins_block).
-          unfold var_inv_preserve.
-          unfold match_temp_env.
-          intros.
-          instantiate (1 := mrs_block) in H0.
-          inversion H1; subst; clear H1.
-          inversion H5; subst; clear H5.
-          inversion H6; subst; clear H6.
-          inversion H7; subst; clear H7.
-          inversion H8; subst; clear H8.
-          inversion H9; subst; clear H9.
-          repeat constructor;auto.
-
-          revert H3. (**r moves the hypotheses  to the goal *)
-          unfold match_elt,fst.
-          destruct (Maps.PTree.get _st le1); try congruence.
-          unfold snd.
-          intro HH ; destruct HH ; split; auto.
-          unfold correct_upd_reg.match_res in H0.
-          unfold stateM_correct in *.
-          tauto.
-        }
-        reflexivity.
-        reflexivity.
-        reflexivity.
-        reflexivity.
-        reflexivity.
-
-        unfold INV; intro H.
-        correct_Forall.
-        get_invariant _st.
-        get_invariant _dst.
-        get_invariant _dst64.
-        get_invariant _src64.
-        destruct c5 as (c5_1 & c5_2).
-        unfold val64_correct,stateless in c5_1.
-        destruct c5_1 as (EQ & (vl1 & VL)); subst.
-        destruct c6 as (c6_1 & c6_2).
-        destruct c6_1 as (EQ & (vl2 & VL)); subst.
-        unfold rBPFValues.val64_divlu, Val.divlu. (**r star here *)
-        unfold rBPFValues.compl_ne, val64_zero in Hdiv_zero.
-        rewrite Bool.negb_true_iff in Hdiv_zero.
-        rewrite Hdiv_zero.
-        exists (v ::v0 :: Vlong (Int64.divu vl1 vl2) :: nil). (**r star here *)
-        unfold map_opt, exec_expr.
-        rewrite p0.
-        rewrite p1. rewrite p2. rewrite p3.
-        split.
-        simpl.
-        unfold Cop.sem_div, Cop.sem_binarith;
-        simpl.
-        Transparent Archi.ptr64.
-        unfold Cop.sem_cast; simpl.
-        rewrite Hdiv_zero.
-        reflexivity.
-        intros.
-        simpl.
-        intuition.
-        unfold stateless,val64_correct.
-        split; auto. eexists ; reflexivity.
-        intros.
-
-        (**r goal: correct_body p unit (returnM tt) fn (Sreturn None) modifies *)
-        eapply correct_body_Sreturn_None.
-        unfold match_res, correct_get_opcode_alu64.match_res.
-        intros.
-        get_invariant _st.
-        destruct c3 as (c3 & _); unfold stateM_correct in c3.
-        destruct c3 as (_ & c3); assumption.
-        reflexivity.
-
-        unfold rBPFValues.compl_ne, val64_zero in Hdiv_zero.
-        (**r goal: correct_body p unit (upd_flag Flag.BPF_ILLEGAL_DIV) fn ... *)
-        eapply correct_statement_seq_body_unit.
-        change_app_for_statement.
-        (**r goal: correct_statement p unit (app f a) fn (Scall None (Evar ... *)
-        eapply correct_statement_call_none.
-        my_reflex.
-        reflexivity.
-        reflexivity.
-        typeclasses eauto.
-        unfold correct_upd_flag.match_res. intuition.
-        { unfold modifies.
-          instantiate (1:= ins_block).
-          unfold var_inv_preserve.
-          unfold match_temp_env.
-          intros.
-          instantiate (1 := mrs_block) in H0.
-          inversion H1; subst; clear H1.
-          inversion H5; subst; clear H5.
-          inversion H6; subst; clear H6.
-          inversion H7; subst; clear H7.
-          inversion H8; subst; clear H8.
-          inversion H9; subst; clear H9.
-          repeat constructor;auto.
-
-          revert H3. (**r moves the hypotheses  to the goal *)
-          unfold match_elt,fst.
-          destruct (Maps.PTree.get _st le1); try congruence.
-          unfold snd.
-          intro HH ; destruct HH ; split; auto.
-          unfold correct_upd_flag.match_res in H0.
-          unfold stateM_correct in *.
-          tauto.
-        }
-        reflexivity.
-        reflexivity.
-        reflexivity.
-        admit.
-        reflexivity.
-
-        unfold INV; intro H.
-        correct_Forall.
-        get_invariant _st.
-        get_invariant _dst.
-        get_invariant _dst64.
-        get_invariant _src64.
-        destruct c5 as (c5_1 & c5_2).
-        unfold val64_correct,stateless in c5_1.
-        destruct c5_1 as (EQ & (vl1 & VL)); subst.
-        destruct c6 as (c6_1 & c6_2).
-        destruct c6_1 as (EQ & (vl2 & VL)); subst.
-        exists (v ::Vint (Int.neg (Int.repr 9)) :: nil). (**r star here *)
-        unfold map_opt, exec_expr.
-        rewrite p0.
-        split.
-        simpl.
-        reflexivity.
-        intros.
-        simpl.
-        intuition.
-        unfold stateless,val64_correct.
-        split; auto.
-        intros.
-
-        (**r goal: correct_body p unit (returnM tt) fn (Sreturn None) modifies *)
-        eapply correct_body_Sreturn_None.
-        unfold match_res, correct_get_opcode_alu64.match_res.
-        intros.
-        get_invariant _st.
-        destruct c3 as (c3 & _); unfold stateM_correct in c3.
-        destruct c3 as (_ & c3); assumption.
-        reflexivity.
-        reflexivity.
-
-        intros.
-        get_invariant _src64.
-        unfold exec_expr.
-        rewrite p0. unfold val64_zero, rBPFValues.compl_ne, Int64.zero.
-        unfold Cop.sem_binary_operation, Cop.sem_cmp, Cop.sem_binarith, Cop.sem_cast; simpl.
-        unfold stateless, val64_correct in c3.
-        destruct c3 as ((c3_0 & c3_vl & c3_1) & c3).
-        subst.
-        reflexivity.
-
-      + reflexivity.
-      + intros.
-        get_invariant _opcode_alu64.
-        unfold exec_expr.
-        rewrite p0. f_equal.
-        unfold correct_get_opcode_alu64.match_res in c3.
-        unfold opcode_alu64_correct in c3.
-        (* opcode_alu64_correct should be a mapping between opcodes and int *)
-        destruct c3; assumption.
-      + compute. intuition congruence. *)
     - (**r op_BPF_RSH64 *)
       admit.
     - (**r op_BPF_NEG64 *)
@@ -1095,7 +905,7 @@ Ltac correct_forward L :=
         reflexivity.
         reflexivity.
         reflexivity.
-        admit. (**r because of Eunop, we could use positve number for bpf_flag *)
+        reflexivity.
         reflexivity.
 
         unfold INV; intro H.
@@ -1166,7 +976,7 @@ Ltac correct_forward L :=
         reflexivity.
         reflexivity.
         reflexivity.
-        admit.
+        reflexivity.
         reflexivity.
 
         unfold INV; intro H.
@@ -1366,7 +1176,7 @@ Ltac correct_forward L :=
         reflexivity.
         reflexivity.
         reflexivity.
-        admit.
+        reflexivity.
         reflexivity.
 
         unfold INV; intro H.
