proof/correctproof/correct_step_opcode_branch.v
@@ -1,0 +1,2014 @@
+From bpf.comm Require Import Regs State Monad.
+From bpf.src Require Import DxNat DxIntegers DxValues DxMonad DxInstructions.
+From Coq Require Import List Lia ZArith.
+From compcert Require Import Integers Values Clight Memory.
+Import ListNotations.
+
+From bpf.proof Require Import Clightlogic MatchState CorrectRel CommonLemma CommonLib CommonLemmaNat.
+
+From bpf.clight Require Import interpreter.
+
+From bpf.proof.correctproof Require Import correct_get_opcode_branch correct_upd_pc
+correct_upd_flag.
+
+(**
+Check step_opcode_branch.
+step_opcode_branch
+     : val64_t ->
+       val64_t -> DxIntegers.sint32_t -> DxIntegers.sint32_t -> nat8 -> M unit
+
+*)
+Open Scope Z_scope.
+
+Section Step_opcode_branch.
+
+  (** The program contains our function of interest [fn] *)
+  Definition p : Clight.program := prog.
+
+  (* [Args,Res] provides the mapping between the Coq and the C types *)
+  (* Definition Args : list CompilableType := [stateCompilableType].*)
+  Definition args : list Type := [(val64_t:Type); (val64_t:Type); (sint32_t:Type); (sint32_t:Type); (nat8:Type)].
+  Definition res : Type := unit.
+
+  (* [f] is a Coq Monadic function with the right type *)
+  Definition f : arrow_type args (M res) := step_opcode_branch.
+
+  Variable state_block: block. (**r a block storing all rbpf state information? *)
+  Variable mrs_block: block.
+  Variable ins_block: block.
+
+  Definition modifies : list block := [state_block]. (* of the C code *)
+
+  Definition stateM_correct (st:unit) (v: val) (stm:State.state) (m: Memory.Mem.mem) :=
+    v = Vptr state_block Ptrofs.zero /\ match_state state_block mrs_block ins_block stm m.
+
+  (* [fn] is the Cligth function which has the same behaviour as [f] *)
+  Definition fn: Clight.function := f_step_opcode_branch.
+
+  (* [match_arg] relates the Coq arguments and the C arguments *)
+  Definition match_arg_list : DList.t (fun x => x -> val -> State.state -> Memory.Mem.mem -> Prop) ((unit:Type) ::args) :=
+    (DList.DCons stateM_correct
+      (DList.DCons (stateless val64_correct)
+       (DList.DCons (stateless val64_correct)
+          (DList.DCons (stateless sint32_correct)
+          (DList.DCons (stateless sint32_correct)
+            (DList.DCons (stateless opcode_alu64_nat8_correct)
+                    (DList.DNil _))))))).
+
+  (* [match_res] relates the Coq result and the C result *)
+  Definition match_res : res -> val -> State.state -> Memory.Mem.mem -> Prop := fun x v st m => match_state state_block mrs_block ins_block st m.
+
+
+Ltac build_app_aux T :=
+  match T with
+  | ?F ?X => let ty := type of X in
+             let r := build_app_aux F in
+             constr:((mk ty X) :: r)
+  | ?X    => constr:(@nil dpair)
+  end.                                    
+
+Ltac get_function T :=
+  match T with
+  | ?F ?X => get_function F
+  | ?X    => X
+  end.
+
+Ltac build_app T :=
+  let a := build_app_aux T in
+  let v := (eval simpl in (DList.of_list_dp (List.rev a))) in
+  let f := get_function T in
+  match type of v with
+  | DList.t _ ?L =>
+      change T with (app (f: arrow_type L _) v)
+  end.
+
+Ltac change_app_for_body :=
+  match goal with
+  | |- @correct_body _ _ ?F _ _ _ _ _ _ _ _
+    => build_app F
+  end.
+
+Ltac change_app_for_statement :=
+  match goal with
+  | |- @correct_statement _ _ ?F _ _ _ _ _ _ _ _
+    => build_app F
+  end.
+
+Ltac prove_incl :=
+  simpl; unfold incl; simpl; intuition congruence.
+
+Ltac prove_in_inv :=
+  simpl; intuition subst; discriminate.
+
+Ltac correct_forward L :=
+  match goal with
+  | |- @correct_body _ _ (bindM ?F1 ?F2)  _
+                     (Ssequence
+                        (Ssequence
+                           (Scall _ _ _)
+                           (Sset ?V ?T))
+                        ?R)
+                     _ _ _ _ _ _  =>
+      eapply L;
+      [ change_app_for_statement ;
+        let b := match T with
+                 | Ecast _ _ => constr:(true)
+                 | _         => constr:(false)
+                 end in
+        eapply correct_statement_call with (has_cast := b)
+      |]
+  | |- @correct_body _ _ (match  ?x with true => _ | false => _ end) _
+                     (Sifthenelse _ _ _)
+                     _ _ _ _ _ _  =>
+      eapply correct_statement_if_body; [prove_in_inv | destruct x ]
+  end.
+
+  Lemma Cop_add : forall vl1 vl2 m,
+       Cop.sem_binary_operation (globalenv p) Cop.Oadd
+                                (Vlong vl1) Clightdefs.tulong (Vlong vl2) Clightdefs.tulong m =
+         Some (Vlong (Int64.add vl1 vl2)).
+  Proof.
+    reflexivity.
+  Qed.
+
+  Instance correct_function3_step_opcode_branch : forall a, correct_function3 p args res f fn modifies false match_arg_list match_res a.
+  Proof.
+    correct_function_from_body args.
+    correct_body.
+
+    unfold f, step_opcode_branch.
+    simpl.
+    (** goal: correct_body _ _ (bindM (get_opcode_branch _) ... *)
+    correct_forward correct_statement_seq_body_nil.
+
+    my_reflex.
+    my_reflex.
+    reflexivity.
+    typeclasses eauto.
+
+    { unfold INV.
+      unfold var_inv_preserve. (**r unmodifies_effect is not enough, we also need unmodifies_effect_state *)
+      intros.
+      unfold match_temp_env in *.
+      rewrite Forall_fold_right in *.
+      simpl in *.
+      destruct H; subst.
+      intuition.
+    }
+
+    reflexivity.
+    reflexivity.
+    reflexivity.
+    prove_in_inv.
+    prove_in_inv.
+    reflexivity.
+    reflexivity.
+
+    unfold INV; intro H.
+    correct_Forall.
+    get_invariant _op.
+    exists (v::nil).
+    split.
+    unfold map_opt. unfold exec_expr. rewrite p0.
+    reflexivity.
+    intros. simpl.
+    tauto.
+
+    (** goal: correct_body _ _
+              match x with
+              | op_BPF_ADD64 => bindM (upd_reg ... *)
+    intros.
+    unfold INV.
+    destruct x eqn: Hbranch. (**r case discussion on each branch_instruction *)
+    - (**r op_BPF_JA *)
+      eapply correct_statement_switch with (n:= 0).
+      + simpl.
+        (**r s1 -> (Ssequence s1 s2) *)
+        eapply correct_statement_seq_body_drop.
+        intros.
+        unfold nat8_0x05.
+        (**r because upd_reg return unit, here we use *_unit? *)
+        eapply correct_statement_if_body_expr.
+
+        destruct (c3 =? 5)%nat eqn: Hneg_eq.
+
+
+        eapply correct_statement_seq_body_unit.
+        change_app_for_statement.
+        (**r goal: correct_statement p unit (app f a) fn (Scall None (Evar ... *)
+        eapply correct_statement_call_none.
+        my_reflex.
+        reflexivity.
+        reflexivity.
+        typeclasses eauto.
+        unfold correct_upd_pc.match_res. intuition.
+        { unfold modifies.
+          instantiate (1:= ins_block).
+          unfold var_inv_preserve.
+          unfold match_temp_env.
+          intros.
+          instantiate (1 := mrs_block) in H0.
+          inversion H1; subst; clear H1.
+          inversion H5; subst; clear H5.
+          inversion H6; subst; clear H6.
+          inversion H7; subst; clear H7.
+          inversion H8; subst; clear H8.
+          inversion H9; subst; clear H9.
+          repeat constructor;auto.
+
+          revert H3. (**r moves the hypotheses  to the goal *)
+          unfold match_elt,fst.
+          destruct (Maps.PTree.get _st le1); try congruence.
+          unfold snd.
+          intro HH ; destruct HH ; split; auto.
+          unfold correct_upd_pc.match_res in H0.
+          unfold stateM_correct in *.
+          tauto.
+          rewrite Forall_forall in H10.
+          apply H10.
+          unfold In. eauto.
+        }
+        reflexivity.
+        reflexivity.
+        reflexivity.
+        reflexivity.
+        reflexivity.
+
+        unfold INV; intro H.
+        correct_Forall.
+        get_invariant _st.
+        get_invariant _pc.
+        get_invariant _ofs.
+        destruct c4 as (c4_1 & c4_2).
+        destruct c5 as (c5_1 & c5_2).
+        unfold sint32_correct,stateless in c5_1, c6.
+        destruct c6 as (c6_1 & c6_2).
+        exists (v :: Vint (Int.add c1 c2) :: nil). (**r star here *)
+        unfold map_opt, exec_expr.
+        rewrite p0.
+        rewrite p1. rewrite p2.
+        split.
+        subst.
+        Transparent Archi.ptr64.
+        unfold Cop.sem_unary_operation, Cop.sem_binary_operation, Cop.sem_add, Cop.classify_add, Cop.sem_binarith, Cop.sem_cast; simpl.
+        reflexivity.
+        intros.
+        simpl.
+        intuition.
+        unfold stateless,sint32_correct.
+        split; auto.
+        intros.
+
+        (**r goal: correct_body p unit (returnM tt) fn (Sreturn None) modifies *)
+        eapply correct_body_Sreturn_None.
+        unfold match_res, correct_get_opcode_branch.match_res.
+        intros.
+        get_invariant _st.
+        destruct c4 as (c4 & _); unfold stateM_correct in c4.
+        destruct c4 as (_ & c4); assumption.
+        reflexivity.
+        eapply correct_statement_seq_body_unit.
+        change_app_for_statement.
+        (**r goal: correct_statement p unit (app f a) fn (Scall None (Evar ... *)
+        eapply correct_statement_call_none.
+        my_reflex.
+        reflexivity.
+        reflexivity.
+        typeclasses eauto.
+        unfold correct_upd_flag.match_res. intuition.
+        { unfold modifies.
+          instantiate (1:= ins_block).
+          unfold var_inv_preserve.
+          unfold match_temp_env.
+          intros.
+          instantiate (1 := mrs_block) in H0.
+          inversion H1; subst; clear H1.
+          inversion H5; subst; clear H5.
+          inversion H6; subst; clear H6.
+          inversion H7; subst; clear H7.
+          inversion H8; subst; clear H8.
+          inversion H9; subst; clear H9.
+          repeat constructor;auto.
+
+          revert H3. (**r moves the hypotheses  to the goal *)
+          unfold match_elt,fst.
+          destruct (Maps.PTree.get _st le1); try congruence.
+          unfold snd.
+          intro HH ; destruct HH ; split; auto.
+          unfold correct_upd_flag.match_res in H0.
+          unfold stateM_correct in *.
+          tauto.
+          rewrite Forall_forall in H10.
+          apply H10.
+          unfold In. eauto.
+        }
+        reflexivity.
+        reflexivity.
+        reflexivity.
+        reflexivity.
+        reflexivity.
+
+        unfold INV; intro H.
+        correct_Forall.
+        get_invariant _st.
+        destruct c4 as (c4_1 & c4_2).
+        exists (v ::Vint (Int.repr (-1)) :: nil). (**r star here: it should be -1 *)
+        unfold map_opt, exec_expr.
+        rewrite p0.
+        split.
+        simpl.
+        reflexivity.
+        intros.
+        simpl.
+        intuition.
+        unfold stateless,flag_correct.
+        unfold int_of_flag; simpl. reflexivity.
+        intros.
+
+        (**r goal: correct_body p unit (returnM tt) fn (Sreturn None) modifies *)
+        eapply correct_body_Sreturn_None.
+        unfold match_res, correct_get_opcode_branch.match_res.
+        intros.
+        get_invariant _st.
+        destruct c4 as (c4 & _); unfold stateM_correct in c4.
+        destruct c4 as (_ & c4); assumption.
+        reflexivity.
+        reflexivity.
+
+        intros.
+        get_invariant _op.
+        unfold exec_expr.
+        rewrite p0. simpl.
+        unfold stateless, opcode_alu64_nat8_correct in c4.
+        destruct c4 as ((Hv_eq & Hland & Hrange) & Hc4).
+        rewrite <- Hv_eq.
+        destruct (c3 =? 5)%nat eqn: Hc2_eq.
+        rewrite Nat.eqb_eq in Hc2_eq.
+        subst.
+        simpl.
+        reflexivity.
+
+        rewrite Nat.eqb_neq in Hc2_eq.
+        simpl.
+        unfold Cop.sem_cmp, Cop.sem_binarith; simpl.
+        assert (Hneq: Int.eq (Int.repr (Z.of_nat c3)) (Int.repr 5) = false). {
+          apply Int.eq_false.
+          apply nat8_neq_5; auto.
+        }
+        rewrite Hneq; clear Hneq.
+        reflexivity.
+      + reflexivity.
+      + intros.
+        get_invariant _opcode_jmp.
+        unfold exec_expr.
+        rewrite p0. f_equal.
+        unfold correct_get_opcode_branch.match_res in c4.
+        unfold opcode_branch_correct in c4.
+        (* opcode_branch_correct should be a mapping between opcodes and int *)
+        destruct c4; assumption.
+      + compute. intuition congruence.
+
+    - (**r op_BPF_JEQ *)
+      eapply correct_statement_switch with (n:= 0x10).
+      + simpl.
+        (**r s1 -> (Ssequence s1 s2) *)
+        eapply correct_statement_seq_body_drop.
+        intros.
+        unfold rBPFValues.compl_eq.
+        (**r because upd_reg return unit, here we use *_unit? *)
+        eapply correct_statement_if_body_expr.
+
+        destruct (match c with
+    | Vlong n1 => match c0 with
+                  | Vlong n2 => Int64.eq n1 n2
+                  | _ => false
+                  end
+    | _ => false
+    end)%nat eqn: Hneg_eq.
+
+
+        eapply correct_statement_seq_body_unit.
+        change_app_for_statement.
+        (**r goal: correct_statement p unit (app f a) fn (Scall None (Evar ... *)
+        eapply correct_statement_call_none.
+        my_reflex.
+        reflexivity.
+        reflexivity.
+        typeclasses eauto.
+        unfold correct_upd_pc.match_res. intuition.
+        { unfold modifies.
+          instantiate (1:= ins_block).
+          unfold var_inv_preserve.
+          unfold match_temp_env.
+          intros.
+          instantiate (1 := mrs_block) in H0.
+          inversion H1; subst; clear H1.
+          inversion H5; subst; clear H5.
+          inversion H6; subst; clear H6.
+          inversion H7; subst; clear H7.
+          inversion H8; subst; clear H8.
+          inversion H9; subst; clear H9.
+          repeat constructor;auto.
+
+          revert H3. (**r moves the hypotheses  to the goal *)
+          unfold match_elt,fst.
+          destruct (Maps.PTree.get _st le1); try congruence.
+          unfold snd.
+          intro HH ; destruct HH ; split; auto.
+          unfold correct_upd_pc.match_res in H0.
+          unfold stateM_correct in *.
+          tauto.
+          rewrite Forall_forall in H10.
+          apply H10.
+          unfold In. eauto.
+        }
+        reflexivity.
+        reflexivity.
+        reflexivity.
+        reflexivity.
+        reflexivity.
+
+        unfold INV; intro H.
+        correct_Forall.
+        get_invariant _st.
+        get_invariant _pc.
+        get_invariant _ofs.
+        destruct c4 as (c4_1 & c4_2).
+        destruct c5 as (c5_1 & c5_2).
+        unfold sint32_correct,stateless in c5_1, c6.
+        destruct c6 as (c6_1 & c6_2).
+        exists (v :: Vint (Int.add c1 c2) :: nil). (**r star here *)
+        unfold map_opt, exec_expr.
+        rewrite p0.
+        rewrite p1. rewrite p2.
+        split.
+        subst.
+        Transparent Archi.ptr64.
+        unfold Cop.sem_unary_operation, Cop.sem_binary_operation, Cop.sem_add, Cop.classify_add, Cop.sem_binarith, Cop.sem_cast; simpl.
+        reflexivity.
+        intros.
+        simpl.
+        intuition.
+        unfold stateless,sint32_correct.
+        split; auto.
+        intros.
+
+        (**r goal: correct_body p unit (returnM tt) fn (Sreturn None) modifies *)
+        eapply correct_body_Sreturn_None.
+        unfold match_res, correct_get_opcode_branch.match_res.
+        intros.
+        get_invariant _st.
+        destruct c4 as (c4 & _); unfold stateM_correct in c4.
+        destruct c4 as (_ & c4); assumption.
+        reflexivity.
+        eapply correct_body_Sreturn_None.
+        unfold match_res, correct_get_opcode_branch.match_res.
+        intros.
+        get_invariant _st.
+        destruct c4 as (c4 & _); unfold stateM_correct in c4.
+        destruct c4 as (_ & c4); assumption.
+        reflexivity.
+        reflexivity.
+        intros.
+        get_invariant _dst64.
+        get_invariant _src64.
+        destruct c4 as (c4 & _); unfold stateless, val64_correct in c4.
+        destruct c4 as (c4_eq & (c4_vl & c4)).
+        destruct c5 as (c5 & _); unfold stateless, val64_correct in c5.
+        destruct c5 as (c5_eq & (c5_vl & c5)).
+        subst.
+        unfold exec_expr.
+        rewrite p0,p1.
+        simpl.
+        reflexivity.
+      + reflexivity.
+      + intros.
+        get_invariant _opcode_jmp.
+        unfold exec_expr.
+        rewrite p0. f_equal.
+        unfold correct_get_opcode_branch.match_res in c4.
+        unfold opcode_branch_correct in c4.
+        (* opcode_branch_correct should be a mapping between opcodes and int *)
+        destruct c4; assumption.
+      + compute. intuition congruence.
+    - (**r op_BPF_JGT *)
+      eapply correct_statement_switch with (n:= 0x20).
+      + simpl.
+        (**r s1 -> (Ssequence s1 s2) *)
+        eapply correct_statement_seq_body_drop.
+        intros.
+        unfold rBPFValues.complu_gt.
+        (**r because upd_reg return unit, here we use *_unit? *)
+        eapply correct_statement_if_body_expr.
+
+        destruct (match c with
+    | Vlong n1 => match c0 with
+                  | Vlong n2 => Int64.ltu n2 n1
+                  | _ => false
+                  end
+    | _ => false
+    end)%nat eqn: Hneg_eq.
+
+
+        eapply correct_statement_seq_body_unit.
+        change_app_for_statement.
+        (**r goal: correct_statement p unit (app f a) fn (Scall None (Evar ... *)
+        eapply correct_statement_call_none.
+        my_reflex.
+        reflexivity.
+        reflexivity.
+        typeclasses eauto.
+        unfold correct_upd_pc.match_res. intuition.
+        { unfold modifies.
+          instantiate (1:= ins_block).
+          unfold var_inv_preserve.
+          unfold match_temp_env.
+          intros.
+          instantiate (1 := mrs_block) in H0.
+          inversion H1; subst; clear H1.
+          inversion H5; subst; clear H5.
+          inversion H6; subst; clear H6.
+          inversion H7; subst; clear H7.
+          inversion H8; subst; clear H8.
+          inversion H9; subst; clear H9.
+          repeat constructor;auto.
+
+          revert H3. (**r moves the hypotheses  to the goal *)
+          unfold match_elt,fst.
+          destruct (Maps.PTree.get _st le1); try congruence.
+          unfold snd.
+          intro HH ; destruct HH ; split; auto.
+          unfold correct_upd_pc.match_res in H0.
+          unfold stateM_correct in *.
+          tauto.
+          rewrite Forall_forall in H10.
+          apply H10.
+          unfold In. eauto.
+        }
+        reflexivity.
+        reflexivity.
+        reflexivity.
+        reflexivity.
+        reflexivity.
+
+        unfold INV; intro H.
+        correct_Forall.
+        get_invariant _st.
+        get_invariant _pc.
+        get_invariant _ofs.
+        destruct c4 as (c4_1 & c4_2).
+        destruct c5 as (c5_1 & c5_2).
+        unfold sint32_correct,stateless in c5_1, c6.
+        destruct c6 as (c6_1 & c6_2).
+        exists (v :: Vint (Int.add c1 c2) :: nil). (**r star here *)
+        unfold map_opt, exec_expr.
+        rewrite p0.
+        rewrite p1. rewrite p2.
+        split.
+        subst.
+        Transparent Archi.ptr64.
+        unfold Cop.sem_unary_operation, Cop.sem_binary_operation, Cop.sem_add, Cop.classify_add, Cop.sem_binarith, Cop.sem_cast; simpl.
+        reflexivity.
+        intros.
+        simpl.
+        intuition.
+        unfold stateless,sint32_correct.
+        split; auto.
+        intros.
+
+        (**r goal: correct_body p unit (returnM tt) fn (Sreturn None) modifies *)
+        eapply correct_body_Sreturn_None.
+        unfold match_res, correct_get_opcode_branch.match_res.
+        intros.
+        get_invariant _st.
+        destruct c4 as (c4 & _); unfold stateM_correct in c4.
+        destruct c4 as (_ & c4); assumption.
+        reflexivity.
+        eapply correct_body_Sreturn_None.
+        unfold match_res, correct_get_opcode_branch.match_res.
+        intros.
+        get_invariant _st.
+        destruct c4 as (c4 & _); unfold stateM_correct in c4.
+        destruct c4 as (_ & c4); assumption.
+        reflexivity.
+        reflexivity.
+        intros.
+        get_invariant _dst64.
+        get_invariant _src64.
+        destruct c4 as (c4 & _); unfold stateless, val64_correct in c4.
+        destruct c4 as (c4_eq & (c4_vl & c4)).
+        destruct c5 as (c5 & _); unfold stateless, val64_correct in c5.
+        destruct c5 as (c5_eq & (c5_vl & c5)).
+        subst.
+        unfold exec_expr.
+        rewrite p0,p1.
+        simpl.
+        reflexivity.
+      + reflexivity.
+      + intros.
+        get_invariant _opcode_jmp.
+        unfold exec_expr.
+        rewrite p0. f_equal.
+        unfold correct_get_opcode_branch.match_res in c4.
+        unfold opcode_branch_correct in c4.
+        (* opcode_branch_correct should be a mapping between opcodes and int *)
+        destruct c4; assumption.
+      + compute. intuition congruence.
+    - (**r op_BPF_JGE *)
+      eapply correct_statement_switch with (n:= 0x30).
+      + simpl.
+        (**r s1 -> (Ssequence s1 s2) *)
+        eapply correct_statement_seq_body_drop.
+        intros.
+        unfold rBPFValues.complu_ge.
+        (**r because upd_reg return unit, here we use *_unit? *)
+        eapply correct_statement_if_body_expr.
+
+        destruct (match c with
+    | Vlong n1 =>
+        match c0 with
+        | Vlong n2 => negb (Int64.ltu n1 n2)
+        | _ => false
+        end
+    | _ => false
+    end)%nat eqn: Hneg_eq.
+
+
+        eapply correct_statement_seq_body_unit.
+        change_app_for_statement.
+        (**r goal: correct_statement p unit (app f a) fn (Scall None (Evar ... *)
+        eapply correct_statement_call_none.
+        my_reflex.
+        reflexivity.
+        reflexivity.
+        typeclasses eauto.
+        unfold correct_upd_pc.match_res. intuition.
+        { unfold modifies.
+          instantiate (1:= ins_block).
+          unfold var_inv_preserve.
+          unfold match_temp_env.
+          intros.
+          instantiate (1 := mrs_block) in H0.
+          inversion H1; subst; clear H1.
+          inversion H5; subst; clear H5.
+          inversion H6; subst; clear H6.
+          inversion H7; subst; clear H7.
+          inversion H8; subst; clear H8.
+          inversion H9; subst; clear H9.
+          repeat constructor;auto.
+
+          revert H3. (**r moves the hypotheses  to the goal *)
+          unfold match_elt,fst.
+          destruct (Maps.PTree.get _st le1); try congruence.
+          unfold snd.
+          intro HH ; destruct HH ; split; auto.
+          unfold correct_upd_pc.match_res in H0.
+          unfold stateM_correct in *.
+          tauto.
+          rewrite Forall_forall in H10.
+          apply H10.
+          unfold In. eauto.
+        }
+        reflexivity.
+        reflexivity.
+        reflexivity.
+        reflexivity.
+        reflexivity.
+
+        unfold INV; intro H.
+        correct_Forall.
+        get_invariant _st.
+        get_invariant _pc.
+        get_invariant _ofs.
+        destruct c4 as (c4_1 & c4_2).
+        destruct c5 as (c5_1 & c5_2).
+        unfold sint32_correct,stateless in c5_1, c6.
+        destruct c6 as (c6_1 & c6_2).
+        exists (v :: Vint (Int.add c1 c2) :: nil). (**r star here *)
+        unfold map_opt, exec_expr.
+        rewrite p0.
+        rewrite p1. rewrite p2.
+        split.
+        subst.
+        Transparent Archi.ptr64.
+        unfold Cop.sem_unary_operation, Cop.sem_binary_operation, Cop.sem_add, Cop.classify_add, Cop.sem_binarith, Cop.sem_cast; simpl.
+        reflexivity.
+        intros.
+        simpl.
+        intuition.
+        unfold stateless,sint32_correct.
+        split; auto.
+        intros.
+
+        (**r goal: correct_body p unit (returnM tt) fn (Sreturn None) modifies *)
+        eapply correct_body_Sreturn_None.
+        unfold match_res, correct_get_opcode_branch.match_res.
+        intros.
+        get_invariant _st.
+        destruct c4 as (c4 & _); unfold stateM_correct in c4.
+        destruct c4 as (_ & c4); assumption.
+        reflexivity.
+        eapply correct_body_Sreturn_None.
+        unfold match_res, correct_get_opcode_branch.match_res.
+        intros.
+        get_invariant _st.
+        destruct c4 as (c4 & _); unfold stateM_correct in c4.
+        destruct c4 as (_ & c4); assumption.
+        reflexivity.
+        reflexivity.
+        intros.
+        get_invariant _dst64.
+        get_invariant _src64.
+        destruct c4 as (c4 & _); unfold stateless, val64_correct in c4.
+        destruct c4 as (c4_eq & (c4_vl & c4)).
+        destruct c5 as (c5 & _); unfold stateless, val64_correct in c5.
+        destruct c5 as (c5_eq & (c5_vl & c5)).
+        subst.
+        unfold exec_expr.
+        rewrite p0,p1.
+        simpl.
+        reflexivity.
+      + reflexivity.
+      + intros.
+        get_invariant _opcode_jmp.
+        unfold exec_expr.
+        rewrite p0. f_equal.
+        unfold correct_get_opcode_branch.match_res in c4.
+        unfold opcode_branch_correct in c4.
+        (* opcode_branch_correct should be a mapping between opcodes and int *)
+        destruct c4; assumption.
+      + compute. intuition congruence.
+    - (**r op_BPF_JLT *)
+      eapply correct_statement_switch with (n:= 0xa0).
+      + simpl.
+        (**r s1 -> (Ssequence s1 s2) *)
+        eapply correct_statement_seq_body_drop.
+        intros.
+        unfold rBPFValues.complu_lt.
+        (**r because upd_reg return unit, here we use *_unit? *)
+        eapply correct_statement_if_body_expr.
+
+        destruct (match c with
+    | Vlong n1 => match c0 with
+                  | Vlong n2 => Int64.ltu n1 n2
+                  | _ => false
+                  end
+    | _ => false
+    end)%nat eqn: Hneg_eq.
+
+
+        eapply correct_statement_seq_body_unit.
+        change_app_for_statement.
+        (**r goal: correct_statement p unit (app f a) fn (Scall None (Evar ... *)
+        eapply correct_statement_call_none.
+        my_reflex.
+        reflexivity.
+        reflexivity.
+        typeclasses eauto.
+        unfold correct_upd_pc.match_res. intuition.
+        { unfold modifies.
+          instantiate (1:= ins_block).
+          unfold var_inv_preserve.
+          unfold match_temp_env.
+          intros.
+          instantiate (1 := mrs_block) in H0.
+          inversion H1; subst; clear H1.
+          inversion H5; subst; clear H5.
+          inversion H6; subst; clear H6.
+          inversion H7; subst; clear H7.
+          inversion H8; subst; clear H8.
+          inversion H9; subst; clear H9.
+          repeat constructor;auto.
+
+          revert H3. (**r moves the hypotheses  to the goal *)
+          unfold match_elt,fst.
+          destruct (Maps.PTree.get _st le1); try congruence.
+          unfold snd.
+          intro HH ; destruct HH ; split; auto.
+          unfold correct_upd_pc.match_res in H0.
+          unfold stateM_correct in *.
+          tauto.
+          rewrite Forall_forall in H10.
+          apply H10.
+          unfold In. eauto.
+        }
+        reflexivity.
+        reflexivity.
+        reflexivity.
+        reflexivity.
+        reflexivity.
+
+        unfold INV; intro H.
+        correct_Forall.
+        get_invariant _st.
+        get_invariant _pc.
+        get_invariant _ofs.
+        destruct c4 as (c4_1 & c4_2).
+        destruct c5 as (c5_1 & c5_2).
+        unfold sint32_correct,stateless in c5_1, c6.
+        destruct c6 as (c6_1 & c6_2).
+        exists (v :: Vint (Int.add c1 c2) :: nil). (**r star here *)
+        unfold map_opt, exec_expr.
+        rewrite p0.
+        rewrite p1. rewrite p2.
+        split.
+        subst.
+        Transparent Archi.ptr64.
+        unfold Cop.sem_unary_operation, Cop.sem_binary_operation, Cop.sem_add, Cop.classify_add, Cop.sem_binarith, Cop.sem_cast; simpl.
+        reflexivity.
+        intros.
+        simpl.
+        intuition.
+        unfold stateless,sint32_correct.
+        split; auto.
+        intros.
+
+        (**r goal: correct_body p unit (returnM tt) fn (Sreturn None) modifies *)
+        eapply correct_body_Sreturn_None.
+        unfold match_res, correct_get_opcode_branch.match_res.
+        intros.
+        get_invariant _st.
+        destruct c4 as (c4 & _); unfold stateM_correct in c4.
+        destruct c4 as (_ & c4); assumption.
+        reflexivity.
+        eapply correct_body_Sreturn_None.
+        unfold match_res, correct_get_opcode_branch.match_res.
+        intros.
+        get_invariant _st.
+        destruct c4 as (c4 & _); unfold stateM_correct in c4.
+        destruct c4 as (_ & c4); assumption.
+        reflexivity.
+        reflexivity.
+        intros.
+        get_invariant _dst64.
+        get_invariant _src64.
+        destruct c4 as (c4 & _); unfold stateless, val64_correct in c4.
+        destruct c4 as (c4_eq & (c4_vl & c4)).
+        destruct c5 as (c5 & _); unfold stateless, val64_correct in c5.
+        destruct c5 as (c5_eq & (c5_vl & c5)).
+        subst.
+        unfold exec_expr.
+        rewrite p0,p1.
+        simpl.
+        reflexivity.
+      + reflexivity.
+      + intros.
+        get_invariant _opcode_jmp.
+        unfold exec_expr.
+        rewrite p0. f_equal.
+        unfold correct_get_opcode_branch.match_res in c4.
+        unfold opcode_branch_correct in c4.
+        (* opcode_branch_correct should be a mapping between opcodes and int *)
+        destruct c4; assumption.
+      + compute. intuition congruence.
+    - (**r op_BPF_JLE *)
+      eapply correct_statement_switch with (n:= 0xb0).
+      + simpl.
+        (**r s1 -> (Ssequence s1 s2) *)
+        eapply correct_statement_seq_body_drop.
+        intros.
+        unfold rBPFValues.complu_le.
+        (**r because upd_reg return unit, here we use *_unit? *)
+        eapply correct_statement_if_body_expr.
+
+        destruct (match c with
+    | Vlong n1 =>
+        match c0 with
+        | Vlong n2 => negb (Int64.ltu n2 n1)
+        | _ => false
+        end
+    | _ => false
+    end)%nat eqn: Hneg_eq.
+
+
+        eapply correct_statement_seq_body_unit.
+        change_app_for_statement.
+        (**r goal: correct_statement p unit (app f a) fn (Scall None (Evar ... *)
+        eapply correct_statement_call_none.
+        my_reflex.
+        reflexivity.
+        reflexivity.
+        typeclasses eauto.
+        unfold correct_upd_pc.match_res. intuition.
+        { unfold modifies.
+          instantiate (1:= ins_block).
+          unfold var_inv_preserve.
+          unfold match_temp_env.
+          intros.
+          instantiate (1 := mrs_block) in H0.
+          inversion H1; subst; clear H1.
+          inversion H5; subst; clear H5.
+          inversion H6; subst; clear H6.
+          inversion H7; subst; clear H7.
+          inversion H8; subst; clear H8.
+          inversion H9; subst; clear H9.
+          repeat constructor;auto.
+
+          revert H3. (**r moves the hypotheses  to the goal *)
+          unfold match_elt,fst.
+          destruct (Maps.PTree.get _st le1); try congruence.
+          unfold snd.
+          intro HH ; destruct HH ; split; auto.
+          unfold correct_upd_pc.match_res in H0.
+          unfold stateM_correct in *.
+          tauto.
+          rewrite Forall_forall in H10.
+          apply H10.
+          unfold In. eauto.
+        }
+        reflexivity.
+        reflexivity.
+        reflexivity.
+        reflexivity.
+        reflexivity.
+
+        unfold INV; intro H.
+        correct_Forall.
+        get_invariant _st.
+        get_invariant _pc.
+        get_invariant _ofs.
+        destruct c4 as (c4_1 & c4_2).
+        destruct c5 as (c5_1 & c5_2).
+        unfold sint32_correct,stateless in c5_1, c6.
+        destruct c6 as (c6_1 & c6_2).
+        exists (v :: Vint (Int.add c1 c2) :: nil). (**r star here *)
+        unfold map_opt, exec_expr.
+        rewrite p0.
+        rewrite p1. rewrite p2.
+        split.
+        subst.
+        Transparent Archi.ptr64.
+        unfold Cop.sem_unary_operation, Cop.sem_binary_operation, Cop.sem_add, Cop.classify_add, Cop.sem_binarith, Cop.sem_cast; simpl.
+        reflexivity.
+        intros.
+        simpl.
+        intuition.
+        unfold stateless,sint32_correct.
+        split; auto.
+        intros.
+
+        (**r goal: correct_body p unit (returnM tt) fn (Sreturn None) modifies *)
+        eapply correct_body_Sreturn_None.
+        unfold match_res, correct_get_opcode_branch.match_res.
+        intros.
+        get_invariant _st.
+        destruct c4 as (c4 & _); unfold stateM_correct in c4.
+        destruct c4 as (_ & c4); assumption.
+        reflexivity.
+        eapply correct_body_Sreturn_None.
+        unfold match_res, correct_get_opcode_branch.match_res.
+        intros.
+        get_invariant _st.
+        destruct c4 as (c4 & _); unfold stateM_correct in c4.
+        destruct c4 as (_ & c4); assumption.
+        reflexivity.
+        reflexivity.
+        intros.
+        get_invariant _dst64.
+        get_invariant _src64.
+        destruct c4 as (c4 & _); unfold stateless, val64_correct in c4.
+        destruct c4 as (c4_eq & (c4_vl & c4)).
+        destruct c5 as (c5 & _); unfold stateless, val64_correct in c5.
+        destruct c5 as (c5_eq & (c5_vl & c5)).
+        subst.
+        unfold exec_expr.
+        rewrite p0,p1.
+        simpl.
+        reflexivity.
+      + reflexivity.
+      + intros.
+        get_invariant _opcode_jmp.
+        unfold exec_expr.
+        rewrite p0. f_equal.
+        unfold correct_get_opcode_branch.match_res in c4.
+        unfold opcode_branch_correct in c4.
+        (* opcode_branch_correct should be a mapping between opcodes and int *)
+        destruct c4; assumption.
+      + compute. intuition congruence.
+    - (**r op_BPF_JSET *)
+      eapply correct_statement_switch with (n:= 0x40).
+      + simpl.
+        (**r s1 -> (Ssequence s1 s2) *)
+        eapply correct_statement_seq_body_drop.
+        intros.
+        unfold rBPFValues.complu_set.
+        (**r because upd_reg return unit, here we use *_unit? *)
+        eapply correct_statement_if_body_expr.
+
+        destruct (match c with
+    | Vlong n1 =>
+        match c0 with
+        | Vlong n2 => negb (Int64.eq (Int64.and n1 n2) Int64.zero)
+        | _ => false
+        end
+    | _ => false
+    end)%nat eqn: Hneg_eq.
+
+
+        eapply correct_statement_seq_body_unit.
+        change_app_for_statement.
+        (**r goal: correct_statement p unit (app f a) fn (Scall None (Evar ... *)
+        eapply correct_statement_call_none.
+        my_reflex.
+        reflexivity.
+        reflexivity.
+        typeclasses eauto.
+        unfold correct_upd_pc.match_res. intuition.
+        { unfold modifies.
+          instantiate (1:= ins_block).
+          unfold var_inv_preserve.
+          unfold match_temp_env.
+          intros.
+          instantiate (1 := mrs_block) in H0.
+          inversion H1; subst; clear H1.
+          inversion H5; subst; clear H5.
+          inversion H6; subst; clear H6.
+          inversion H7; subst; clear H7.
+          inversion H8; subst; clear H8.
+          inversion H9; subst; clear H9.
+          repeat constructor;auto.
+
+          revert H3. (**r moves the hypotheses  to the goal *)
+          unfold match_elt,fst.
+          destruct (Maps.PTree.get _st le1); try congruence.
+          unfold snd.
+          intro HH ; destruct HH ; split; auto.
+          unfold correct_upd_pc.match_res in H0.
+          unfold stateM_correct in *.
+          tauto.
+          rewrite Forall_forall in H10.
+          apply H10.
+          unfold In. eauto.
+        }
+        reflexivity.
+        reflexivity.
+        reflexivity.
+        reflexivity.
+        reflexivity.
+
+        unfold INV; intro H.
+        correct_Forall.
+        get_invariant _st.
+        get_invariant _pc.
+        get_invariant _ofs.
+        destruct c4 as (c4_1 & c4_2).
+        destruct c5 as (c5_1 & c5_2).
+        unfold sint32_correct,stateless in c5_1, c6.
+        destruct c6 as (c6_1 & c6_2).
+        exists (v :: Vint (Int.add c1 c2) :: nil). (**r star here *)
+        unfold map_opt, exec_expr.
+        rewrite p0.
+        rewrite p1. rewrite p2.
+        split.
+        subst.
+        Transparent Archi.ptr64.
+        unfold Cop.sem_unary_operation, Cop.sem_binary_operation, Cop.sem_add, Cop.classify_add, Cop.sem_binarith, Cop.sem_cast; simpl.
+        reflexivity.
+        intros.
+        simpl.
+        intuition.
+        unfold stateless,sint32_correct.
+        split; auto.
+        intros.
+
+        (**r goal: correct_body p unit (returnM tt) fn (Sreturn None) modifies *)
+        eapply correct_body_Sreturn_None.
+        unfold match_res, correct_get_opcode_branch.match_res.
+        intros.
+        get_invariant _st.
+        destruct c4 as (c4 & _); unfold stateM_correct in c4.
+        destruct c4 as (_ & c4); assumption.
+        reflexivity.
+        eapply correct_body_Sreturn_None.
+        unfold match_res, correct_get_opcode_branch.match_res.
+        intros.
+        get_invariant _st.
+        destruct c4 as (c4 & _); unfold stateM_correct in c4.
+        destruct c4 as (_ & c4); assumption.
+        reflexivity.
+        reflexivity.
+        intros.
+        get_invariant _dst64.
+        get_invariant _src64.
+        destruct c4 as (c4 & _); unfold stateless, val64_correct in c4.
+        destruct c4 as (c4_eq & (c4_vl & c4)).
+        destruct c5 as (c5 & _); unfold stateless, val64_correct in c5.
+        destruct c5 as (c5_eq & (c5_vl & c5)).
+        subst.
+        unfold exec_expr.
+        rewrite p0,p1.
+        simpl.
+        reflexivity.
+      + reflexivity.
+      + intros.
+        get_invariant _opcode_jmp.
+        unfold exec_expr.
+        rewrite p0. f_equal.
+        unfold correct_get_opcode_branch.match_res in c4.
+        unfold opcode_branch_correct in c4.
+        (* opcode_branch_correct should be a mapping between opcodes and int *)
+        destruct c4; assumption.
+      + compute. intuition congruence.
+    - (**r op_BPF_JNE *)
+      eapply correct_statement_switch with (n:= 0x50).
+      + simpl.
+        (**r s1 -> (Ssequence s1 s2) *)
+        eapply correct_statement_seq_body_drop.
+        intros.
+        unfold rBPFValues.compl_ne.
+        (**r because upd_reg return unit, here we use *_unit? *)
+        eapply correct_statement_if_body_expr.
+
+        destruct (match c with
+    | Vlong n1 =>
+        match c0 with
+        | Vlong n2 => negb (Int64.eq n1 n2)
+        | _ => false
+        end
+    | _ => false
+    end)%nat eqn: Hneg_eq.
+
+
+        eapply correct_statement_seq_body_unit.
+        change_app_for_statement.
+        (**r goal: correct_statement p unit (app f a) fn (Scall None (Evar ... *)
+        eapply correct_statement_call_none.
+        my_reflex.
+        reflexivity.
+        reflexivity.
+        typeclasses eauto.
+        unfold correct_upd_pc.match_res. intuition.
+        { unfold modifies.
+          instantiate (1:= ins_block).
+          unfold var_inv_preserve.
+          unfold match_temp_env.
+          intros.
+          instantiate (1 := mrs_block) in H0.
+          inversion H1; subst; clear H1.
+          inversion H5; subst; clear H5.
+          inversion H6; subst; clear H6.
+          inversion H7; subst; clear H7.
+          inversion H8; subst; clear H8.
+          inversion H9; subst; clear H9.
+          repeat constructor;auto.
+
+          revert H3. (**r moves the hypotheses  to the goal *)
+          unfold match_elt,fst.
+          destruct (Maps.PTree.get _st le1); try congruence.
+          unfold snd.
+          intro HH ; destruct HH ; split; auto.
+          unfold correct_upd_pc.match_res in H0.
+          unfold stateM_correct in *.
+          tauto.
+          rewrite Forall_forall in H10.
+          apply H10.
+          unfold In. eauto.
+        }
+        reflexivity.
+        reflexivity.
+        reflexivity.
+        reflexivity.
+        reflexivity.
+
+        unfold INV; intro H.
+        correct_Forall.
+        get_invariant _st.
+        get_invariant _pc.
+        get_invariant _ofs.
+        destruct c4 as (c4_1 & c4_2).
+        destruct c5 as (c5_1 & c5_2).
+        unfold sint32_correct,stateless in c5_1, c6.
+        destruct c6 as (c6_1 & c6_2).
+        exists (v :: Vint (Int.add c1 c2) :: nil). (**r star here *)
+        unfold map_opt, exec_expr.
+        rewrite p0.
+        rewrite p1. rewrite p2.
+        split.
+        subst.
+        Transparent Archi.ptr64.
+        unfold Cop.sem_unary_operation, Cop.sem_binary_operation, Cop.sem_add, Cop.classify_add, Cop.sem_binarith, Cop.sem_cast; simpl.
+        reflexivity.
+        intros.
+        simpl.
+        intuition.
+        unfold stateless,sint32_correct.
+        split; auto.
+        intros.
+
+        (**r goal: correct_body p unit (returnM tt) fn (Sreturn None) modifies *)
+        eapply correct_body_Sreturn_None.
+        unfold match_res, correct_get_opcode_branch.match_res.
+        intros.
+        get_invariant _st.
+        destruct c4 as (c4 & _); unfold stateM_correct in c4.
+        destruct c4 as (_ & c4); assumption.
+        reflexivity.
+        eapply correct_body_Sreturn_None.
+        unfold match_res, correct_get_opcode_branch.match_res.
+        intros.
+        get_invariant _st.
+        destruct c4 as (c4 & _); unfold stateM_correct in c4.
+        destruct c4 as (_ & c4); assumption.
+        reflexivity.
+        reflexivity.
+        intros.
+        get_invariant _dst64.
+        get_invariant _src64.
+        destruct c4 as (c4 & _); unfold stateless, val64_correct in c4.
+        destruct c4 as (c4_eq & (c4_vl & c4)).
+        destruct c5 as (c5 & _); unfold stateless, val64_correct in c5.
+        destruct c5 as (c5_eq & (c5_vl & c5)).
+        subst.
+        unfold exec_expr.
+        rewrite p0,p1.
+        simpl.
+        reflexivity.
+      + reflexivity.
+      + intros.
+        get_invariant _opcode_jmp.
+        unfold exec_expr.
+        rewrite p0. f_equal.
+        unfold correct_get_opcode_branch.match_res in c4.
+        unfold opcode_branch_correct in c4.
+        (* opcode_branch_correct should be a mapping between opcodes and int *)
+        destruct c4; assumption.
+      + compute. intuition congruence.
+    - (**r op_BPF_JSGT *)
+      eapply correct_statement_switch with (n:= 0x60).
+      + simpl.
+        (**r s1 -> (Ssequence s1 s2) *)
+        eapply correct_statement_seq_body_drop.
+        intros.
+        unfold rBPFValues.compl_gt.
+        (**r because upd_reg return unit, here we use *_unit? *)
+        eapply correct_statement_if_body_expr.
+
+        destruct (match c with
+    | Vlong n1 => match c0 with
+                  | Vlong n2 => Int64.lt n2 n1
+                  | _ => false
+                  end
+    | _ => false
+    end)%nat eqn: Hneg_eq.
+
+
+        eapply correct_statement_seq_body_unit.
+        change_app_for_statement.
+        (**r goal: correct_statement p unit (app f a) fn (Scall None (Evar ... *)
+        eapply correct_statement_call_none.
+        my_reflex.
+        reflexivity.
+        reflexivity.
+        typeclasses eauto.
+        unfold correct_upd_pc.match_res. intuition.
+        { unfold modifies.
+          instantiate (1:= ins_block).
+          unfold var_inv_preserve.
+          unfold match_temp_env.
+          intros.
+          instantiate (1 := mrs_block) in H0.
+          inversion H1; subst; clear H1.
+          inversion H5; subst; clear H5.
+          inversion H6; subst; clear H6.
+          inversion H7; subst; clear H7.
+          inversion H8; subst; clear H8.
+          inversion H9; subst; clear H9.
+          repeat constructor;auto.
+
+          revert H3. (**r moves the hypotheses  to the goal *)
+          unfold match_elt,fst.
+          destruct (Maps.PTree.get _st le1); try congruence.
+          unfold snd.
+          intro HH ; destruct HH ; split; auto.
+          unfold correct_upd_pc.match_res in H0.
+          unfold stateM_correct in *.
+          tauto.
+          rewrite Forall_forall in H10.
+          apply H10.
+          unfold In. eauto.
+        }
+        reflexivity.
+        reflexivity.
+        reflexivity.
+        reflexivity.
+        reflexivity.
+
+        unfold INV; intro H.
+        correct_Forall.
+        get_invariant _st.
+        get_invariant _pc.
+        get_invariant _ofs.
+        destruct c4 as (c4_1 & c4_2).
+        destruct c5 as (c5_1 & c5_2).
+        unfold sint32_correct,stateless in c5_1, c6.
+        destruct c6 as (c6_1 & c6_2).
+        exists (v :: Vint (Int.add c1 c2) :: nil). (**r star here *)
+        unfold map_opt, exec_expr.
+        rewrite p0.
+        rewrite p1. rewrite p2.
+        split.
+        subst.
+        Transparent Archi.ptr64.
+        unfold Cop.sem_unary_operation, Cop.sem_binary_operation, Cop.sem_add, Cop.classify_add, Cop.sem_binarith, Cop.sem_cast; simpl.
+        reflexivity.
+        intros.
+        simpl.
+        intuition.
+        unfold stateless,sint32_correct.
+        split; auto.
+        intros.
+
+        (**r goal: correct_body p unit (returnM tt) fn (Sreturn None) modifies *)
+        eapply correct_body_Sreturn_None.
+        unfold match_res, correct_get_opcode_branch.match_res.
+        intros.
+        get_invariant _st.
+        destruct c4 as (c4 & _); unfold stateM_correct in c4.
+        destruct c4 as (_ & c4); assumption.
+        reflexivity.
+        eapply correct_body_Sreturn_None.
+        unfold match_res, correct_get_opcode_branch.match_res.
+        intros.
+        get_invariant _st.
+        destruct c4 as (c4 & _); unfold stateM_correct in c4.
+        destruct c4 as (_ & c4); assumption.
+        reflexivity.
+        reflexivity.
+        intros.
+        get_invariant _dst64.
+        get_invariant _src64.
+        destruct c4 as (c4 & _); unfold stateless, val64_correct in c4.
+        destruct c4 as (c4_eq & (c4_vl & c4)).
+        destruct c5 as (c5 & _); unfold stateless, val64_correct in c5.
+        destruct c5 as (c5_eq & (c5_vl & c5)).
+        subst.
+        unfold exec_expr.
+        rewrite p0,p1.
+        simpl.
+        reflexivity.
+      + reflexivity.
+      + intros.
+        get_invariant _opcode_jmp.
+        unfold exec_expr.
+        rewrite p0. f_equal.
+        unfold correct_get_opcode_branch.match_res in c4.
+        unfold opcode_branch_correct in c4.
+        (* opcode_branch_correct should be a mapping between opcodes and int *)
+        destruct c4; assumption.
+      + compute. intuition congruence.
+    - (**r op_BPF_JSGE *)
+      eapply correct_statement_switch with (n:= 0x70).
+      + simpl.
+        (**r s1 -> (Ssequence s1 s2) *)
+        eapply correct_statement_seq_body_drop.
+        intros.
+        unfold rBPFValues.compl_ge.
+        (**r because upd_reg return unit, here we use *_unit? *)
+        eapply correct_statement_if_body_expr.
+
+        destruct (match c with
+    | Vlong n1 =>
+        match c0 with
+        | Vlong n2 => negb (Int64.lt n1 n2)
+        | _ => false
+        end
+    | _ => false
+    end)%nat eqn: Hneg_eq.
+
+
+        eapply correct_statement_seq_body_unit.
+        change_app_for_statement.
+        (**r goal: correct_statement p unit (app f a) fn (Scall None (Evar ... *)
+        eapply correct_statement_call_none.
+        my_reflex.
+        reflexivity.
+        reflexivity.
+        typeclasses eauto.
+        unfold correct_upd_pc.match_res. intuition.
+        { unfold modifies.
+          instantiate (1:= ins_block).
+          unfold var_inv_preserve.
+          unfold match_temp_env.
+          intros.
+          instantiate (1 := mrs_block) in H0.
+          inversion H1; subst; clear H1.
+          inversion H5; subst; clear H5.
+          inversion H6; subst; clear H6.
+          inversion H7; subst; clear H7.
+          inversion H8; subst; clear H8.
+          inversion H9; subst; clear H9.
+          repeat constructor;auto.
+
+          revert H3. (**r moves the hypotheses  to the goal *)
+          unfold match_elt,fst.
+          destruct (Maps.PTree.get _st le1); try congruence.
+          unfold snd.
+          intro HH ; destruct HH ; split; auto.
+          unfold correct_upd_pc.match_res in H0.
+          unfold stateM_correct in *.
+          tauto.
+          rewrite Forall_forall in H10.
+          apply H10.
+          unfold In. eauto.
+        }
+        reflexivity.
+        reflexivity.
+        reflexivity.
+        reflexivity.
+        reflexivity.
+
+        unfold INV; intro H.
+        correct_Forall.
+        get_invariant _st.
+        get_invariant _pc.
+        get_invariant _ofs.
+        destruct c4 as (c4_1 & c4_2).
+        destruct c5 as (c5_1 & c5_2).
+        unfold sint32_correct,stateless in c5_1, c6.
+        destruct c6 as (c6_1 & c6_2).
+        exists (v :: Vint (Int.add c1 c2) :: nil). (**r star here *)
+        unfold map_opt, exec_expr.
+        rewrite p0.
+        rewrite p1. rewrite p2.
+        split.
+        subst.
+        Transparent Archi.ptr64.
+        unfold Cop.sem_unary_operation, Cop.sem_binary_operation, Cop.sem_add, Cop.classify_add, Cop.sem_binarith, Cop.sem_cast; simpl.
+        reflexivity.
+        intros.
+        simpl.
+        intuition.
+        unfold stateless,sint32_correct.
+        split; auto.
+        intros.
+
+        (**r goal: correct_body p unit (returnM tt) fn (Sreturn None) modifies *)
+        eapply correct_body_Sreturn_None.
+        unfold match_res, correct_get_opcode_branch.match_res.
+        intros.
+        get_invariant _st.
+        destruct c4 as (c4 & _); unfold stateM_correct in c4.
+        destruct c4 as (_ & c4); assumption.
+        reflexivity.
+        eapply correct_body_Sreturn_None.
+        unfold match_res, correct_get_opcode_branch.match_res.
+        intros.
+        get_invariant _st.
+        destruct c4 as (c4 & _); unfold stateM_correct in c4.
+        destruct c4 as (_ & c4); assumption.
+        reflexivity.
+        reflexivity.
+        intros.
+        get_invariant _dst64.
+        get_invariant _src64.
+        destruct c4 as (c4 & _); unfold stateless, val64_correct in c4.
+        destruct c4 as (c4_eq & (c4_vl & c4)).
+        destruct c5 as (c5 & _); unfold stateless, val64_correct in c5.
+        destruct c5 as (c5_eq & (c5_vl & c5)).
+        subst.
+        unfold exec_expr.
+        rewrite p0,p1.
+        simpl.
+        reflexivity.
+      + reflexivity.
+      + intros.
+        get_invariant _opcode_jmp.
+        unfold exec_expr.
+        rewrite p0. f_equal.
+        unfold correct_get_opcode_branch.match_res in c4.
+        unfold opcode_branch_correct in c4.
+        (* opcode_branch_correct should be a mapping between opcodes and int *)
+        destruct c4; assumption.
+      + compute. intuition congruence.
+    - (**r op_BPF_JSLT *)
+      eapply correct_statement_switch with (n:= 0xc0).
+      + simpl.
+        (**r s1 -> (Ssequence s1 s2) *)
+        eapply correct_statement_seq_body_drop.
+        intros.
+        unfold rBPFValues.compl_lt.
+        (**r because upd_reg return unit, here we use *_unit? *)
+        eapply correct_statement_if_body_expr.
+
+        destruct (match c with
+    | Vlong n1 => match c0 with
+                  | Vlong n2 => Int64.lt n1 n2
+                  | _ => false
+                  end
+    | _ => false
+    end)%nat eqn: Hneg_eq.
+
+
+        eapply correct_statement_seq_body_unit.
+        change_app_for_statement.
+        (**r goal: correct_statement p unit (app f a) fn (Scall None (Evar ... *)
+        eapply correct_statement_call_none.
+        my_reflex.
+        reflexivity.
+        reflexivity.
+        typeclasses eauto.
+        unfold correct_upd_pc.match_res. intuition.
+        { unfold modifies.
+          instantiate (1:= ins_block).
+          unfold var_inv_preserve.
+          unfold match_temp_env.
+          intros.
+          instantiate (1 := mrs_block) in H0.
+          inversion H1; subst; clear H1.
+          inversion H5; subst; clear H5.
+          inversion H6; subst; clear H6.
+          inversion H7; subst; clear H7.
+          inversion H8; subst; clear H8.
+          inversion H9; subst; clear H9.
+          repeat constructor;auto.
+
+          revert H3. (**r moves the hypotheses  to the goal *)
+          unfold match_elt,fst.
+          destruct (Maps.PTree.get _st le1); try congruence.
+          unfold snd.
+          intro HH ; destruct HH ; split; auto.
+          unfold correct_upd_pc.match_res in H0.
+          unfold stateM_correct in *.
+          tauto.
+          rewrite Forall_forall in H10.
+          apply H10.
+          unfold In. eauto.
+        }
+        reflexivity.
+        reflexivity.
+        reflexivity.
+        reflexivity.
+        reflexivity.
+
+        unfold INV; intro H.
+        correct_Forall.
+        get_invariant _st.
+        get_invariant _pc.
+        get_invariant _ofs.
+        destruct c4 as (c4_1 & c4_2).
+        destruct c5 as (c5_1 & c5_2).
+        unfold sint32_correct,stateless in c5_1, c6.
+        destruct c6 as (c6_1 & c6_2).
+        exists (v :: Vint (Int.add c1 c2) :: nil). (**r star here *)
+        unfold map_opt, exec_expr.
+        rewrite p0.
+        rewrite p1. rewrite p2.
+        split.
+        subst.
+        Transparent Archi.ptr64.
+        unfold Cop.sem_unary_operation, Cop.sem_binary_operation, Cop.sem_add, Cop.classify_add, Cop.sem_binarith, Cop.sem_cast; simpl.
+        reflexivity.
+        intros.
+        simpl.
+        intuition.
+        unfold stateless,sint32_correct.
+        split; auto.
+        intros.
+
+        (**r goal: correct_body p unit (returnM tt) fn (Sreturn None) modifies *)
+        eapply correct_body_Sreturn_None.
+        unfold match_res, correct_get_opcode_branch.match_res.
+        intros.
+        get_invariant _st.
+        destruct c4 as (c4 & _); unfold stateM_correct in c4.
+        destruct c4 as (_ & c4); assumption.
+        reflexivity.
+        eapply correct_body_Sreturn_None.
+        unfold match_res, correct_get_opcode_branch.match_res.
+        intros.
+        get_invariant _st.
+        destruct c4 as (c4 & _); unfold stateM_correct in c4.
+        destruct c4 as (_ & c4); assumption.
+        reflexivity.
+        reflexivity.
+        intros.
+        get_invariant _dst64.
+        get_invariant _src64.
+        destruct c4 as (c4 & _); unfold stateless, val64_correct in c4.
+        destruct c4 as (c4_eq & (c4_vl & c4)).
+        destruct c5 as (c5 & _); unfold stateless, val64_correct in c5.
+        destruct c5 as (c5_eq & (c5_vl & c5)).
+        subst.
+        unfold exec_expr.
+        rewrite p0,p1.
+        simpl.
+        reflexivity.
+      + reflexivity.
+      + intros.
+        get_invariant _opcode_jmp.
+        unfold exec_expr.
+        rewrite p0. f_equal.
+        unfold correct_get_opcode_branch.match_res in c4.
+        unfold opcode_branch_correct in c4.
+        (* opcode_branch_correct should be a mapping between opcodes and int *)
+        destruct c4; assumption.
+      + compute. intuition congruence.
+    - (**r op_BPF_JSLE *)
+      eapply correct_statement_switch with (n:= 0xd0).
+      + simpl.
+        (**r s1 -> (Ssequence s1 s2) *)
+        eapply correct_statement_seq_body_drop.
+        intros.
+        unfold rBPFValues.compl_le.
+        (**r because upd_reg return unit, here we use *_unit? *)
+        eapply correct_statement_if_body_expr.
+
+        destruct (match c with
+    | Vlong n1 =>
+        match c0 with
+        | Vlong n2 => negb (Int64.lt n2 n1)
+        | _ => false
+        end
+    | _ => false
+    end)%nat eqn: Hneg_eq.
+
+
+        eapply correct_statement_seq_body_unit.
+        change_app_for_statement.
+        (**r goal: correct_statement p unit (app f a) fn (Scall None (Evar ... *)
+        eapply correct_statement_call_none.
+        my_reflex.
+        reflexivity.
+        reflexivity.
+        typeclasses eauto.
+        unfold correct_upd_pc.match_res. intuition.
+        { unfold modifies.
+          instantiate (1:= ins_block).
+          unfold var_inv_preserve.
+          unfold match_temp_env.
+          intros.
+          instantiate (1 := mrs_block) in H0.
+          inversion H1; subst; clear H1.
+          inversion H5; subst; clear H5.
+          inversion H6; subst; clear H6.
+          inversion H7; subst; clear H7.
+          inversion H8; subst; clear H8.
+          inversion H9; subst; clear H9.
+          repeat constructor;auto.
+
+          revert H3. (**r moves the hypotheses  to the goal *)
+          unfold match_elt,fst.
+          destruct (Maps.PTree.get _st le1); try congruence.
+          unfold snd.
+          intro HH ; destruct HH ; split; auto.
+          unfold correct_upd_pc.match_res in H0.
+          unfold stateM_correct in *.
+          tauto.
+          rewrite Forall_forall in H10.
+          apply H10.
+          unfold In. eauto.
+        }
+        reflexivity.
+        reflexivity.
+        reflexivity.
+        reflexivity.
+        reflexivity.
+
+        unfold INV; intro H.
+        correct_Forall.
+        get_invariant _st.
+        get_invariant _pc.
+        get_invariant _ofs.
+        destruct c4 as (c4_1 & c4_2).
+        destruct c5 as (c5_1 & c5_2).
+        unfold sint32_correct,stateless in c5_1, c6.
+        destruct c6 as (c6_1 & c6_2).
+        exists (v :: Vint (Int.add c1 c2) :: nil). (**r star here *)
+        unfold map_opt, exec_expr.
+        rewrite p0.
+        rewrite p1. rewrite p2.
+        split.
+        subst.
+        Transparent Archi.ptr64.
+        unfold Cop.sem_unary_operation, Cop.sem_binary_operation, Cop.sem_add, Cop.classify_add, Cop.sem_binarith, Cop.sem_cast; simpl.
+        reflexivity.
+        intros.
+        simpl.
+        intuition.
+        unfold stateless,sint32_correct.
+        split; auto.
+        intros.
+
+        (**r goal: correct_body p unit (returnM tt) fn (Sreturn None) modifies *)
+        eapply correct_body_Sreturn_None.
+        unfold match_res, correct_get_opcode_branch.match_res.
+        intros.
+        get_invariant _st.
+        destruct c4 as (c4 & _); unfold stateM_correct in c4.
+        destruct c4 as (_ & c4); assumption.
+        reflexivity.
+        eapply correct_body_Sreturn_None.
+        unfold match_res, correct_get_opcode_branch.match_res.
+        intros.
+        get_invariant _st.
+        destruct c4 as (c4 & _); unfold stateM_correct in c4.
+        destruct c4 as (_ & c4); assumption.
+        reflexivity.
+        reflexivity.
+        intros.
+        get_invariant _dst64.
+        get_invariant _src64.
+        destruct c4 as (c4 & _); unfold stateless, val64_correct in c4.
+        destruct c4 as (c4_eq & (c4_vl & c4)).
+        destruct c5 as (c5 & _); unfold stateless, val64_correct in c5.
+        destruct c5 as (c5_eq & (c5_vl & c5)).
+        subst.
+        unfold exec_expr.
+        rewrite p0,p1.
+        simpl.
+        reflexivity.
+      + reflexivity.
+      + intros.
+        get_invariant _opcode_jmp.
+        unfold exec_expr.
+        rewrite p0. f_equal.
+        unfold correct_get_opcode_branch.match_res in c4.
+        unfold opcode_branch_correct in c4.
+        (* opcode_branch_correct should be a mapping between opcodes and int *)
+        destruct c4; assumption.
+      + compute. intuition congruence.
+    - (**r op_BPF_RET *)
+
+      eapply correct_statement_switch with (n:= 0x90).
+      + simpl.
+        (**r s1 -> (Ssequence s1 s2) *)
+        eapply correct_statement_seq_body_drop.
+        intros.
+        unfold nat8_0x95.
+        (**r because upd_reg return unit, here we use *_unit? *)
+
+        eapply correct_statement_if_body_expr.
+
+        destruct (c3 =? 149)%nat eqn: Hneg_eq.
+
+
+        eapply correct_statement_seq_body_unit.
+        change_app_for_statement.
+        (**r goal: correct_statement p unit (app f a) fn (Scall None (Evar ... *)
+        eapply correct_statement_call_none.
+        my_reflex.
+        reflexivity.
+        reflexivity.
+        typeclasses eauto.
+        unfold correct_upd_flag.match_res. intuition.
+        { unfold modifies.
+          instantiate (1:= ins_block).
+          unfold var_inv_preserve.
+          unfold match_temp_env.
+          intros.
+          instantiate (1 := mrs_block) in H0.
+          inversion H1; subst; clear H1.
+          inversion H5; subst; clear H5.
+          inversion H6; subst; clear H6.
+          inversion H7; subst; clear H7.
+          inversion H8; subst; clear H8.
+          inversion H9; subst; clear H9.
+          repeat constructor;auto.
+
+          revert H3. (**r moves the hypotheses  to the goal *)
+          unfold match_elt,fst.
+          destruct (Maps.PTree.get _st le1); try congruence.
+          unfold snd.
+          intro HH ; destruct HH ; split; auto.
+          unfold correct_upd_flag.match_res in H0.
+          unfold stateM_correct in *.
+          destruct H1, H0.
+          split; assumption.
+          rewrite Forall_forall in H10.
+          apply H10.
+          unfold In. eauto.
+        }
+        reflexivity.
+        reflexivity.
+        reflexivity.
+        reflexivity.
+        reflexivity.
+
+        unfold INV; intro H.
+        correct_Forall.
+        get_invariant _st.
+        get_invariant _pc.
+        get_invariant _ofs.
+        destruct c4 as (c4_1 & c4_2).
+        destruct c5 as (c5_1 & c5_2).
+        unfold sint32_correct,stateless in c5_1, c6.
+        destruct c6 as (c6_1 & c6_2).
+        exists (v :: Vint (Int.repr 1) :: nil). (**r star here *)
+        unfold map_opt, exec_expr.
+        rewrite p0.
+        split. reflexivity.
+        subst.
+        intros.
+        simpl.
+        intuition.
+        unfold stateless,flag_correct, int_of_flag.
+        split; auto.
+        intros.
+
+        (**r goal: correct_body p unit (returnM tt) fn (Sreturn None) modifies *)
+        eapply correct_body_Sreturn_None.
+        unfold match_res, correct_get_opcode_branch.match_res.
+        intros.
+        get_invariant _st.
+        destruct c4 as (c4 & _); unfold stateM_correct in c4.
+        destruct c4 as (_ & c4); assumption.
+        reflexivity.
+        eapply correct_statement_seq_body_unit.
+        change_app_for_statement.
+        (**r goal: correct_statement p unit (app f a) fn (Scall None (Evar ... *)
+        eapply correct_statement_call_none.
+        my_reflex.
+        reflexivity.
+        reflexivity.
+        typeclasses eauto.
+        unfold correct_upd_flag.match_res. intuition.
+        { unfold modifies.
+          instantiate (1:= ins_block).
+          unfold var_inv_preserve.
+          unfold match_temp_env.
+          intros.
+          instantiate (1 := mrs_block) in H0.
+          inversion H1; subst; clear H1.
+          inversion H5; subst; clear H5.
+          inversion H6; subst; clear H6.
+          inversion H7; subst; clear H7.
+          inversion H8; subst; clear H8.
+          inversion H9; subst; clear H9.
+          repeat constructor;auto.
+
+          revert H3. (**r moves the hypotheses  to the goal *)
+          unfold match_elt,fst.
+          destruct (Maps.PTree.get _st le1); try congruence.
+          unfold snd.
+          intro HH ; destruct HH ; split; auto.
+          unfold correct_upd_flag.match_res in H0.
+          unfold stateM_correct in *.
+          tauto.
+          rewrite Forall_forall in H10.
+          apply H10.
+          unfold In. eauto.
+        }
+        reflexivity.
+        reflexivity.
+        reflexivity.
+        reflexivity.
+        reflexivity.
+
+        unfold INV; intro H.
+        correct_Forall.
+        get_invariant _st.
+        destruct c4 as (c4_1 & c4_2).
+        exists (v ::Vint (Int.repr (-1)) :: nil). (**r star here: it should be -1 *)
+        unfold map_opt, exec_expr.
+        rewrite p0.
+        split.
+        simpl.
+        reflexivity.
+        intros.
+        simpl.
+        intuition.
+        unfold stateless,flag_correct.
+        unfold int_of_flag; simpl. reflexivity.
+        intros.
+
+        (**r goal: correct_body p unit (returnM tt) fn (Sreturn None) modifies *)
+        eapply correct_body_Sreturn_None.
+        unfold match_res, correct_get_opcode_branch.match_res.
+        intros.
+        get_invariant _st.
+        destruct c4 as (c4 & _); unfold stateM_correct in c4.
+        destruct c4 as (_ & c4); assumption.
+        reflexivity.
+        reflexivity.
+
+        intros.
+        get_invariant _op.
+        unfold exec_expr.
+        rewrite p0. simpl.
+        unfold stateless, opcode_alu64_nat8_correct in c4.
+        destruct c4 as ((Hv_eq & Hland & Hrange) & Hc4).
+        rewrite <- Hv_eq.
+        destruct (c3 =? 149)%nat eqn: Hc2_eq.
+        rewrite Nat.eqb_eq in Hc2_eq.
+        subst.
+        simpl.
+        reflexivity.
+
+        rewrite Nat.eqb_neq in Hc2_eq.
+        simpl.
+        unfold Cop.sem_cmp, Cop.sem_binarith; simpl.
+        assert (Hneq: Int.eq (Int.repr (Z.of_nat c3)) (Int.repr 149) = false). {
+          apply Int.eq_false.
+          apply nat8_neq_149; auto.
+        }
+        rewrite Hneq; clear Hneq.
+        reflexivity.
+      + reflexivity.
+      + intros.
+        get_invariant _opcode_jmp.
+        unfold exec_expr.
+        rewrite p0. f_equal.
+        unfold correct_get_opcode_branch.match_res in c4.
+        unfold opcode_branch_correct in c4.
+        (* opcode_branch_correct should be a mapping between opcodes and int *)
+        destruct c4; assumption.
+      + compute. intuition congruence.
+
+    - (**r op_BPF_JMP_ILLEGAL_INS *)
+      admit.
+(*
+      eapply correct_statement_switch with (n:= 1).
+      + simpl.
+        (**r s1 -> (Ssequence s1 s2) *)
+        eapply correct_statement_seq_body_drop.
+        intros.
+
+        eapply correct_statement_seq_body_unit.
+        change_app_for_statement.
+        (**r goal: correct_statement p unit (app f a) fn (Scall None (Evar ... *)
+        eapply correct_statement_call_none.
+        my_reflex.
+        reflexivity.
+        reflexivity.
+        typeclasses eauto.
+        unfold correct_upd_flag.match_res. intuition.
+        { unfold modifies.
+          instantiate (1:= ins_block).
+          unfold var_inv_preserve.
+          unfold match_temp_env.
+          intros.
+          instantiate (1 := mrs_block) in H0.
+          inversion H1; subst; clear H1.
+          inversion H5; subst; clear H5.
+          inversion H6; subst; clear H6.
+          inversion H7; subst; clear H7.
+          inversion H8; subst; clear H8.
+          inversion H9; subst; clear H9.
+          repeat constructor;auto.
+
+          revert H3. (**r moves the hypotheses  to the goal *)
+          unfold match_elt,fst.
+          destruct (Maps.PTree.get _st le1); try congruence.
+          unfold snd.
+          intro HH ; destruct HH ; split; auto.
+          unfold correct_upd_flag.match_res in H0.
+          unfold stateM_correct in *.
+          destruct H1, H0.
+          split; assumption.
+          rewrite Forall_forall in H10.
+          apply H10.
+          unfold In. eauto.
+        }
+        reflexivity.
+        reflexivity.
+        reflexivity.
+        reflexivity.
+        reflexivity.
+
+        unfold INV; intro H.
+        correct_Forall.
+        get_invariant _st.
+        get_invariant _pc.
+        get_invariant _ofs.
+        destruct c4 as (c4_1 & c4_2).
+        destruct c5 as (c5_1 & c5_2).
+        unfold sint32_correct,stateless in c5_1, c6.
+        destruct c6 as (c6_1 & c6_2).
+        exists (v :: Vint (Int.repr (-1)) :: nil). (**r star here *)
+        unfold map_opt, exec_expr.
+        rewrite p0.
+        split. reflexivity.
+        subst.
+        intros.
+        simpl.
+        intuition.
+        unfold stateless,flag_correct, int_of_flag.
+        split; auto.
+        intros.
+
+        (**r goal: correct_body p unit (returnM tt) fn (Sreturn None) modifies *)
+        eapply correct_body_Sreturn_None.
+        unfold match_res, correct_get_opcode_branch.match_res.
+        intros.
+        get_invariant _st.
+        destruct c4 as (c4 & _); unfold stateM_correct in c4.
+        destruct c4 as (_ & c4); assumption.
+        reflexivity.
+      + reflexivity.
+      + intros.
+        get_invariant _opcode_jmp.
+        unfold exec_expr.
+        rewrite p0. f_equal.
+        unfold correct_get_opcode_branch.match_res in c4.
+        unfold opcode_branch_correct in c4.
+        (* opcode_branch_correct should be a mapping between opcodes and int *)
+        destruct c4. assumption.
+      + compute. intuition congruence.*)
+
+Admitted.
+
+End Step_opcode_branch.
+
+Close Scope Z_scope.
+
+Existing Instance correct_function3_step_opcode_branch.
